{
  "@context": {
    "dcterms": "http://purl.org/dc/terms/",
    "owl": "http://www.w3.org/2002/07/owl#",
    "rdf": "http://www.w3.org/1999/02/22-rdf-syntax-ns#",
    "rdfs": "http://www.w3.org/2000/01/rdf-schema#",
    "schema": "https://schema.org/",
    "sh": "http://www.w3.org/ns/shacl#",
    "skos": "http://www.w3.org/2004/02/skos/core#",
    "xsd": "http://www.w3.org/2001/XMLSchema#",
	"data": "http://jellyfiiish.xyz/ns/"
  },
  "@graph": [
	{
      "@id": "data:Document",
      "@type": "rdfs:Class",
      "skos:definition": "A piece of written, printed, or electronic material that provides information.",
	  "rdfs:comment": ["A document is often based on some document template.", "A document typically serves as a record of some event, such as a meeting, an application or a request."]
      "rdfs:label": "Document",
      "rdfs:subClassOf": {
        "@id": "dcterms:Resource"
      }
    },
	{
      "@id": "data:resourceContent",
      "@type": "rdf:Property",
      "skos:definition": "The actual content of a dcterms:Resource.",
      "rdfs:label": "resourceContent",
      "schema:domainIncludes": {
        "@id": "dcterms:Resource"
      },
      "schema:rangeIncludes": {
        "@id": "TODO: Anything."
      },
	  "rdfs:comment": "If the actual content of the resource cannot be provided via this property, it should be provided via the data:resourceContentLocation property."
    },
	{
      "@id": "data:resourceContentLocation",
      "@type": "rdf:Property",
      "skos:definition": "The location, whether online or offline, of the content of the resource.",
      "rdfs:label": "resourceContent",
      "schema:domainIncludes": {
        "@id": "dcterms:Resource"
      },
      "schema:rangeIncludes": {
        "@id": "TODO."
      },
	  "rdfs:comment": "Should be provided if the actual content of the resource cannot be provided via the data:resourceContent property."
    },
	{
      "@id": "data:versionTag",
      "@type": "rdf:Property",
      "skos:definition": "A textual indentifier for a specific version of a resource.",
      "rdfs:label": "versionTag",
      "schema:domainIncludes": {
        "@id": "dcterms:Resource"
      },
      "schema:rangeIncludes": {
        "@id": "xsd:string"
      },
	  "rdfs:comment": "E.g., '1.4.2'"
    }
	
]
