{
  "@context": {
    "dcterms": "http://purl.org/dc/terms/",
    "owl": "http://www.w3.org/2002/07/owl#",
    "rdf": "http://www.w3.org/1999/02/22-rdf-syntax-ns#",
    "rdfs": "http://www.w3.org/2000/01/rdf-schema#",
    "schema": "https://schema.org/",
    "sh": "http://www.w3.org/ns/shacl#",
    "skos": "http://www.w3.org/2004/02/skos/core#",
    "xsd": "http://www.w3.org/2001/XMLSchema#",
	"data": "http://jellyfiiish.xyz/ns/"
  },
  "@graph": [
	{
      "@id": "data:Datum",
      "@type": "rdfs:Class",
      "skos:definition": "A single piece (or 'atom') of information. In relational database terms it is a single cell in a table, i.e., the intersection of a row (entity) and a column (attribute); in graph database terms it is two nodes connected by an arc; in document terms it is typically the response to a single document field; in RDF terms it is a single semantic triple (i.e., a subject, a predicate and an object).",
      "rdfs:label": "Datum",
	  "rdfs:comment": "'Data' is the plural of 'datum', i.e., it is multiple atoms of information. It is an uncountable noun (like money) and therefore takes the singular form of a verb (i.e., 'data is...', not 'data are...').",
      "rdfs:subClassOf": {
        "@id": "dcterms:Resource"
      }
    },
	{
      "@id": "data:Dataset",
      "@type": "rdfs:Class",
      "skos:definition": "A collection of data that forms some conceptual whole.",
      "rdfs:label": "Dataset",
	  "rdfs:comment": "The data in a dataset typically has a single, common source.",
      "rdfs:subClassOf": {
        "@id": "dcterms:Resource"
      }
    },
	{
      "@id": "data:Document",
      "@type": "rdfs:Class",
      "skos:definition": "A piece of written, printed, or electronic material that provides information.",
	  "rdfs:comment": [
		"A document is often based on some document template.", 
		"A document typically serves as a record of some event, such as a meeting, an application or a request."
	  ],
      "rdfs:label": "Document",
      "rdfs:subClassOf": {
        "@id": "dcterms:Resource"
      }
    },
	{
      "@id": "data:resourceContent",
      "@type": "rdf:Property",
      "skos:definition": "The actual content of a dcterms:Resource.",
      "rdfs:label": "resourceContent",
      "schema:domainIncludes": {
        "@id": "dcterms:Resource"
      },
      "schema:rangeIncludes": {
        "@id": "owl:Thing"
      },
	  "rdfs:comment": "If the actual content of the resource cannot be provided via this property, it should be provided via the data:resourceContentLocation property."
    },
	{
      "@id": "data:resourceContentLocation",
      "@type": "rdf:Property",
      "skos:definition": "The location, whether online or offline, of the content of the resource.",
      "rdfs:label": "resourceContent",
      "schema:domainIncludes": {
        "@id": "dcterms:Resource"
      },
      "schema:rangeIncludes": {
        "@id": "schema:Text"
      },
	  "rdfs:comment": "Should be provided if the actual content of the resource cannot be provided via the data:resourceContent property."
    },
	{
      "@id": "data:versionTag",
      "@type": "rdf:Property",
      "skos:definition": "A textual indentifier for a specific version of a resource.",
      "rdfs:label": "versionTag",
      "schema:domainIncludes": {
        "@id": "dcterms:Resource"
      },
      "schema:rangeIncludes": {
        "@id": "xsd:string"
      },
	  "rdfs:comment": "E.g., '1.4.2'"
    },
	{
      "@id": "data:DataAction",
      "@type": "rdfs:Class",
      "skos:definition": "Any action (e.g., observation, collection, retrieval, cleaning, anonymisation, transformation, or aggregation) performed on data or a datum that created or altered it in terms of content, shape, structure, identifiability or any other conceivable way.",
	  "rdfs:comment": "A dataset typically goes through a process of creation (through the observation of some phenomemnon), quality control, correction, anonymisation, etc., resulting in different versions of the dataset.",
      "rdfs:label": "DataAction",
      "rdfs:subClassOf": {
        "@id": "owl:Thing"
      }
    },
	{
      "@id": "data:input",
      "@type": "rdf:Property",
      "skos:definition": "The input to a data action, i.e., the resource (datum, dataset, document, etc.) being acted upon.",
      "rdfs:label": "input",
      "schema:domainIncludes": [
		{ "@id": "data:DataAction" },
	  ],
      "schema:rangeIncludes": {
        "@id": "dcterms:Resource"
      },
	  "rdfs:comment": "It is the resource in its state prior to the action in question."
    },
	{
      "@id": "data:output",
      "@type": "rdf:Property",
      "skos:definition": "The output of a data action, i.e., the resulting resource (datum, dataset, document, etc.).",
      "rdfs:label": "output",
      "schema:domainIncludes": [
		{ "@id": "data:DataAction" },
	  ],
      "schema:rangeIncludes": {
        "@id": "dcterms:Resource"
      },
	  "rdfs:comment": "It is the resource in its state directly after the action in question."
    },
	{
      "@id": "data:instrument",
      "@type": "rdf:Property",
      "skos:definition": "The instrument with which a data action is performed.",
      "rdfs:label": "instrument",
      "schema:domainIncludes": [
		{ "@id": "data:DataAction" },
	  ],
      "schema:rangeIncludes": {
        "@id": "owl:Thing"
      },
	  "skos:example": [
		"A sensor that collects data.",
		"A questionnaire used by a fieldworker.",
		"An R script that reshapes a dataset."
	  ]
    },
	{
      "@id": "data:report",
      "@type": "rdf:Property",
      "skos:definition": "A detailed description of a data action and its result(s).",
      "rdfs:label": "report",
      "schema:domainIncludes": [
		{ "@id": "data:DataAction" },
	  ],
      "schema:rangeIncludes": {
        "@id": "dcterms:Resource",
		"@id": "schema:Text"
      }
    },
	{
      "@id": "data:lineage",
      "@type": "rdf:Property",
      "skos:definition": "A series of data actions that explains how a (specific version of a) dataset or other resource came into being.",
      "rdfs:label": "lineage",
      "schema:domainIncludes": [
		{ "@id": "dcterms:Resource" },
	  ],
      "schema:rangeIncludes": {
        "@id": "data:DataAction"
      }
    }
  ]
}
